feat: remove the Dot notation from Coq

CoqOfRust/_std/fs.v
@@ -20,28 +20,24 @@ Require CoqOfRust._std.path.
 Module FileTimes.
   Parameter t : Set.
 End FileTimes.
-Definition FileTimes := FileTimes.t.
 
 (* pub struct DirBuilder { /* private fields */ } *)
 Module DirBuilder.
   Parameter t : Set.
 End DirBuilder.
-Definition DirBuilder := DirBuilder.t.
 
 (* pub struct DirEntry(_); *)
 Module DirEntry.
   Parameter t : Set.
 End DirEntry.
-Definition DirEntry := DirEntry.t.
 
 (* pub struct File { /* private fields */ } *)
 Module File.
   Parameter t : Set.
 End File.
-Definition File := File.t.
 
 Module Impl_Write_for_File.
-  Global Instance I : _std.io.Write.Trait File.
+  Global Instance I : _std.io.Write.Trait File.t.
   Admitted.
 End Impl_Write_for_File.
 
@@ -49,22 +45,19 @@ End Impl_Write_for_File.
 Module FileType.
   Parameter t : Set.
 End FileType.
-Definition FileType := FileType.t.
 
 (* pub struct Metadata(_); *)
 Module Metadata.
   Parameter t : Set.
 End Metadata.
-Definition Metadata := Metadata.t.
 
 (* pub struct OpenOptions(_); *)
 Module OpenOptions.
   Parameter t : Set.
 End OpenOptions.
-Definition OpenOptions : Set := OpenOptions.t.
 
 Module Impl_OpenOptions.
-  Definition Self := OpenOptions.
+  Definition Self := OpenOptions.t.
 
   Parameter new : M Self.
 
@@ -76,73 +69,35 @@ Module Impl_OpenOptions.
   Parameter read :
     mut_ref Self -> bool -> M (mut_ref Self).
 
-  Global Instance Method_read :
-    Notations.Dot "read" := {
-    Notations.dot := read;
-  }.
-
   Parameter write :
     mut_ref Self -> bool -> M (mut_ref Self).
-
-  Global Instance Method_write :
-    Notations.Dot "write" := {
-    Notations.dot := write;
-  }.
 
   Parameter append :
     mut_ref Self -> bool -> M (mut_ref Self).
 
-  Global Instance Method_append :
-    Notations.Dot "append" := {
-    Notations.dot := append;
-  }.
-
   Parameter truncate :
     mut_ref Self -> bool -> M (mut_ref Self).
-
-  Global Instance Method_truncate :
-    Notations.Dot "truncate" := {
-    Notations.dot := truncate;
-  }.
 
   Parameter create :
     mut_ref Self -> bool -> M (mut_ref Self).
 
-  Global Instance Method_create :
-    Notations.Dot "create" := {
-    Notations.dot := create;
-  }.
-
   Parameter create_new :
     mut_ref Self -> bool -> M (mut_ref Self).
 
-  Global Instance Method_create_new :
-    Notations.Dot "create_new" := {
-    Notations.dot := create_new;
-  }.
-
   Parameter open :
     forall {P : Set} (*`{core.convert.AsRef.Trait P _std.path.Path}*),
-    ref Self -> P -> M (_std.io.Result File).
-
-  Global Instance Method_open {P : Set}
-      (*`{core.convert.AsRef.Trait P _std.path.Path}*) :
-    Notations.Dot "open" := {
-    Notations.dot := open (P := P);
-  }.
+    ref Self -> P -> M (_std.io.Result File.t).
 End Impl_OpenOptions.
 
 (* pub struct Permissions(_); *)
 Module Permissions.
   Parameter t : Set.
 End Permissions.
-Definition Permissions := Permissions.t.
 
 (* pub struct ReadDir(_); *)
 Module ReadDir.
   Parameter t : Set.
 End ReadDir.
-Definition ReadDir := ReadDir.t.
 
 (* ********FUNCTIONS******** *)
 (*
